add caml types

theories/Interpreter.v
@@ -1,12 +1,12 @@
 Require Import ssreflect.
 
-Require Import ZArith Array.PArray List Floats Lia.
+Require Import ZArith Array.PArray List String Floats Lia.
+Require Ascii.
+Require Uint63.
 Import ListNotations.
 
-(*Require Import Malfunction.Malfunction Malfunction.Deserialize Malfunction.SemanticsSpec Malfunction.Serialize Ceres.Ceres.*)
-
-Require Import Malfunction.Malfunction Malfunction.SemanticsSpec Malfunction.utils_array.
-From MetaCoq.Utils Require Import bytestring.
+Require Import Malfunction.Malfunction Malfunction.Deserialize Malfunction.SemanticsSpec Malfunction.Serialize Ceres.Ceres.
+From MetaCoq Require Import bytestring.
 Open Scope bs.
 
 From Coq Require Import Uint63.
@@ -106,6 +106,20 @@ Definition truncate `{Heap} ty n :=
                      if Z.ltb masked min_int then masked else
                        Z.sub masked range
                  end).
+
+#[bypass_check(guard)]
+Fixpoint to_sexp_value (a : value) : sexp :=
+  match a with
+  | Block (i, a) => @Serialize_product _ _ _ (@Serialize_list _ to_sexp_value) (i, List.map (fun j => a.[int_of_nat j]) (seq 0 (int_to_nat (PArray.length a))))
+  | Vec x => Atom "TODO VEC"
+  | Func x => Atom "FUNC"
+  | value_Int x => Atom "TODO INT"
+  | Float x => Atom "TODO FLOAT"
+  | Thunk x => Atom "THUNK"
+  | fail x => Atom ("fail" ++ String.to_string x)
+  end%string.
+
+#[export] Instance Serialize_value : Serialize value := to_sexp_value.
 
 #[bypass_check(guard)]
 Fixpoint interpret `{Heap} (h : heap)
